DY/Bytes/AttackerKnowledgeTheorem.lean
@@ -13,6 +13,7 @@ public import DY.Bytes.Invariants
 public import DY.Bytes.AttackerKnowledge
 import all DY.Bytes.AttackerKnowledge
 public import DY.Trace
+public meta import DY.Meta.CombineMacro
 
 namespace DY
 
@@ -81,5 +82,55 @@ theorem Bytes.AttackerKnows_implies_Publishable
     assumption
 
 grind_pattern Bytes.AttackerKnows_implies_Publishable => Bytes.AttackerKnows b tr.erase
+
+namespace Meta.CombineMacro
+
+macro_rules
+  | `(command| #combine_one $options* SubAttackerKnowledgeTheorem $params* from $sources,*) => do
+    let options := parseOptions options
+    let baseGlobalInstances := #[
+      (← `(bracketedBinder| [DY.BytesFunctor])),
+      (← `(bracketedBinder| [DY.ExecTraceTypes])),
+      (← `(bracketedBinder| [DY.ProofTraceTypes])),
+      (← `(bracketedBinder| [DY.TraceInvariant])),
+      (← `(bracketedBinder| [DY.BytesInvariants])),
+    ]
+    let params := if options.toplevel then params else baseGlobalInstances ++ params
+    let sources := sources.getElems
+
+    let combined ← combineTypeclass params sources <| .makeSimple {
+      refereeName := `attackerKnowledge
+      combineName := ``DY.SubAttackerKnowledge.combine
+      outTypeName := ``DY.SubAttackerKnowledgeTheorem
+    }
+
+    let attStx := Lean.mkIdent `attackerKnowledge
+    let topLevelInst ← `(command| public instance: DY.AttackerKnowledgeTheorem where inst := inferInstanceAs (DY.SubAttackerKnowledgeTheorem $attStx))
+    let topLevel := if options.toplevel then #[topLevelInst] else #[]
+
+    return Lean.mkNullNode (combined ++ topLevel)
+
+macro_rules
+  | `(command| #combine_one $_options* SubAttackerKnowledgeTheorem' $params* from $sources,*) => do
+    -- options.toplevel does not make sense in this case, hence we ignore it
+    let baseGlobalInstances := #[
+      (← `(bracketedBinder| [DY.BytesFunctor])),
+      (← `(bracketedBinder| [DY.ExecTraceTypes])),
+      (← `(bracketedBinder| [DY.ProofTraceTypes])),
+      (← `(bracketedBinder| [DY.TraceInvariant])),
+      (← `(bracketedBinder| [DY.BytesInvariants])),
+    ]
+    let params := baseGlobalInstances ++ params
+    let sources := sources.getElems
+
+    let combined ← combineTypeclass params sources <| .makeSimple {
+      refereeName := `attackerKnowledge
+      combineName := ``DY.SubAttackerKnowledge.combine'
+      outTypeName := ``DY.SubAttackerKnowledgeTheorem
+    }
+
+    return Lean.mkNullNode (combined)
+
+end Meta.CombineMacro
 
 end DY
