DY/Trace/BaseAttackerKnowledgeTheorem.lean
@@ -7,6 +7,7 @@ public import DY.Trace.Invariant
 public import DY.Trace.BaseAttackerKnowledge
 import all DY.Trace.Invariant
 import all DY.Trace.BaseAttackerKnowledge
+public meta import DY.Meta.CombineMacro
 
 namespace DY
 
@@ -74,5 +75,73 @@ theorem Trace.BaseAttackerKnows_implies_Publishable
   · have := BaseAttackerKnowledgeTheorem.pf.pf trBefore entry b (by grind [ProofTrace.Entry.Invariant]) (by grind [ProofTrace.Entry.erase])
     grind
   · grind
+
+namespace Meta.CombineMacro
+
+macro_rules
+  | `(command| #combine_one $options* SubBaseAttackerKnowledgeTheorem__expertMode $params* from $sources,*) => do
+    let options := parseOptions options
+    let proofInternalStx := Lean.mkIdent `ProofEntryT.internal
+    let proofStx := Lean.mkIdent `ProofEntryT
+    let baseAttInternalStx := Lean.mkIdent `baseAttackerKnowledge.internal
+    let baseAttStx := Lean.mkIdent `baseAttackerKnowledge
+
+    let baseGlobalInstances := #[
+      (← `(bracketedBinder| [DY.ExecTraceTypes])),
+      (← `(bracketedBinder| [DY.ProofTraceTypes])),
+      (← `(bracketedBinder| [DY.BytesFunctor])),
+      (← `(bracketedBinder| [DY.TraceInvariant])),
+      (← `(bracketedBinder| [DY.BytesInvariants])),
+    ]
+
+    let params := if options.toplevel then params else baseGlobalInstances ++ params
+
+    let sources := sources.getElems
+
+    let combined ← combineTypeclass params sources {
+      internalIdStx args id := `(term| DY.SubBaseAttackerKnowledgeTheorem ($proofInternalStx $args* $id) ($baseAttInternalStx $args* $id))
+      internalStx name args := do
+        let internalProofStx := Lean.mkIdentFrom name <| name.getId.modifyBase (. ++ `ProofEntryT)
+        let internalBaseAttStx := Lean.mkIdentFrom name <| name.getId.modifyBase (. ++ `baseAttackerKnowledge)
+        `(term| DY.SubBaseAttackerKnowledgeTheorem ($internalProofStx $args*) ($internalBaseAttStx $args*))
+      combineStx args := `(term| DY.SubBaseAttackerKnowledgeTheorem (DY.ProofTraceTypes.combine ($proofInternalStx $args*)) (DY.SubBaseAttackerKnowledge.combine ($baseAttInternalStx $args*)))
+      finalStx args := `(term| DY.SubBaseAttackerKnowledgeTheorem ($proofStx $args*) ($baseAttStx $args*))
+      useInferInstanceAs := false
+    }
+
+    let topLevelInst ← `(command| public instance: DY.BaseAttackerKnowledgeTheorem where pf := inferInstanceAs (DY.SubBaseAttackerKnowledgeTheorem $proofStx $baseAttStx))
+    let topLevel := if options.toplevel then #[topLevelInst] else #[]
+
+    return Lean.mkNullNode (combined ++ topLevel)
+
+macro_rules
+  | `(command| #combine_one $options* SubBaseAttackerKnowledgeTheorem__noExecHas $params* from $sources,*) => do
+    let proofStx := Lean.mkIdent `ProofEntryT
+
+    let argsTarget := params.flatMap explicitNameOfBracketedBinder
+    let hasInstances := #[
+      (← `(bracketedBinder| [DY.ProofTraceTypes.Has ($proofStx $argsTarget*)])),
+      (← `(bracketedBinder| [DY.TraceInvariant.Has ($proofStx $argsTarget*)]))
+    ]
+    `(command| #combine_one $options* SubBaseAttackerKnowledgeTheorem__expertMode $params* $hasInstances* from $sources,*)
+
+macro_rules
+  | `(command| #combine_one $options* SubBaseAttackerKnowledgeTheorem $params* from $sources,*) => do
+    let opts := parseOptions options
+    let execStx := Lean.mkIdent `ExecEntryT
+    let proofStx := Lean.mkIdent `ProofEntryT
+
+    let argsTarget := params.flatMap explicitNameOfBracketedBinder
+    let hasInstances := #[
+      (← `(bracketedBinder| [DY.ExecTraceTypes.Has ($execStx $argsTarget*)])),
+      (← `(bracketedBinder| [DY.ProofTraceTypes.Has ($proofStx $argsTarget*)])),
+      (← `(bracketedBinder| [DY.TraceInvariant.Has ($proofStx $argsTarget*)]))
+    ]
+
+    let params := if opts.toplevel then params else params ++ hasInstances
+
+    `(command| #combine_one $options* SubBaseAttackerKnowledgeTheorem__expertMode $params* from $sources,*)
+
+end Meta.CombineMacro
 
 end DY
